\documentclass[11pt]{article}

\input{./defs.tex}

\begin{document}

\hwtitle
  {Assignment 1}
  {Isaak Yansane-Sisk}

\problem{Problem 1}
    \begin{enumerate}
        \item 
            $ \fun{x}{x} $ \par
            Already in $\beta$-normal form.
        \item $ \fun{x}{y} $ \par
        Contains a free-variable but is nonetheless a valid lambda term ($ \val{e} $) in $\beta$-normal form.
        \item  $ x $ \par
        A single free variable is not defined in our semantics so this is a 'stuck state' ($ \not\exists e' . \steps{e}{e'} $ ) but a valid value.
        \item $(\app{\fun{x}{\fun{y}{x}}}{y})(\app{\fun{y}{y}}{y}) \mapsto \app{\fun{y}{y}}{y} \mapsto y $
        \item $(\app{\fun{x}{x}}{x})(\app{\fun{x}{x}}{x}) \mapsto (\app{\app{\fun{x}{x}}{x}}){x} \mapsto \app{x}{x}$ \par
        This is an invalid (or "stuck") value, no way to apply a free variable to another ($\neg(\val{e})$).
        \item $ (\app{\app{\fun{x}{\fun{x}{x}}){a}}}{b} \equiv_\alpha (\app{\app{\fun{x}{\fun{y}{y}}){a}}}{b} \mapsto \app{\fun{y}{y}}{b} \mapsto b $
        \item $\app{(\fun{x}{\fun{y}{x}})}{z} \mapsto z $
    \end{enumerate}


\problem{Problem 3}

Your answer goes here. Here's the dynamically-scoped untyped lambda calculus operational semantics as examples of writing inference rules.

\begin{mathpar}
\ir{V-Lam}{ \ }{\val{\fun{x}{e}}}

\ir{D-Var}
  {\ctx(x) = e}
  {\dynJC{\steps{x}{e}}}

\ir{D-App$_1$}
  {\dynJC{\steps{e_1}{e_1'}}}
  {\dynJC{\steps{\app{e_1}{e_2}}{\app{e_1'}{e_2}}}}

\ir{D-App$_2$}
  {\dynJ{\ctx, x \rightarrow e_2}{\steps{e_1}{e_1'}}}
  {\dynJC{\steps{\app{(\fun{x}{e_1})}{e_2}}{\app{(\fun{x}{e_1'})}{e_2}}}}

\ir{D-App$_3$}
  {\val{e_1}}
  {\dynJC{\steps{\app{(\fun{x}{e_1})}{e_2}}{e_1}}}
\end{mathpar}

\begin{mathpar}
\text{Step 1:}\qquad
\ir{D-App$_2$}
  {\ir{D-App$_1$}
    {\ir{D-App$_3$}
      {\ir{D-Lam}{ \ }{\val{\fun{\_}{x}}}}
      {\dynJ{\{x \rightarrow D\}}{\steps
        {\app{(\fun{x}{\fun{\_}{x}})}{L}}
        {\fun{\_}{x}}}}}
    {\dynJ{\{x \rightarrow D\}}{\steps
      {\app{\app{(\fun{x}{\fun{\_}{x}})}{L}}{*}}
      {\app{(\fun{\_}{x})}{*}}}}}
  {\dynJ{\varnothing}{\steps
    {\app{(\fun{x}{\app{\app{(\fun{x}{\fun{\_}{x}})}{L}}{*}})}{D}}
    {\app{(\fun{x}{\app{(\fun{\_}{x})}{*}})}{D}}}}
\end{mathpar}

\begin{mathpar}
\text{Step 2:}\qquad
\ir{D-App$_2$}
  {\ir{D-App$_2$}
    {\ir{D-Var}
      {\ctx(x) = D}
      {\dynJ{\{x \rightarrow D, \_ \rightarrow *\}}{\steps{x}{D}}}}
    {\dynJ{\{x \rightarrow D\}}{\steps{\app{(\fun{\_}{x})}{*}}}{D}}}
  {\dynJ{\varnothing}{\steps
  {\app{(\app{\fun{x}{(\fun{\_}{x})}}{*})}{D}}
  {(\app{\fun{x}{x})}{D}}}}
\end{mathpar}

\begin{mathpar}
\text{Step 3:}\qquad
\ir{D-App$_2$}
  {\ir{D-Var}
    {\ctx(x) = D}
    {\dynJ{\{x \rightarrow D\}}{\steps{x}{D}}}}
  {\dynJ{\varnothing}{\steps
    {\app{(\fun{x}{x})}{D}}
    {\app{(\fun{x}{D})}{D}}}}
\end{mathpar}

\begin{mathpar}
\text{Step 4:}\qquad
\ir{D-App$_3$}
  {\val{D}}
  {\steps
    {\app{(\fun{x}{D})}{D}}
    {D}}
\end{mathpar}

\end{document}
